rewrote proof of soundness of new superposition proof obligation.

unitb/refinement/superposition.lean
@@ -30,11 +30,14 @@ structure evt_ref_wk (lbl : Type) (mc : program α') (ea : event α) (ecs : lbl 
   (witness : lbl → α' → Prop)
   (sim : ∀ ec, ⟦ (ecs ec).step_of ⟧ ⟹ ⟦ ea.step_of on abs ⟧)
   (delay : (ea.coarse_sch && ea.fine_sch) ∘ abs
-            ↦
+            >~>
            -(ea.coarse_sch ∘ abs)
-            || ∃∃ ec, witness ec && (ecs ec).coarse_sch && (ecs ec).fine_sch in mc)
+            || ∃∃ ec, witness ec && (ecs ec).coarse_sch in mc)
   (stable : ∀ ec, unless_except mc (witness ec && (ecs ec).coarse_sch) (-(ea.coarse_sch ∘ abs))
                                    { e | ∃ l, ecs l = e })
+  (resched : ∀ ec, (ea.coarse_sch && ea.fine_sch) ∘ abs && witness ec && (ecs ec).coarse_sch
+                    >~>
+                   (ecs ec).fine_sch in mc)
 
 lemma evt_ref_wk_of_evt_ref
   (lbl : Type) (mc : program α')
@@ -57,9 +60,9 @@ begin
         rw [p_and_comm,p_or_self,p_and_comm] at H',
         apply H', },
       have P₁ : H.witness ec && (ecs ec).coarse_sch || (ecs ec).fine_sch
-               ↦
-              -(ea.coarse_sch ∘ abs)
-              || H.witness ec && (ecs ec).coarse_sch && (ecs ec).fine_sch in mc,
+                 ↦
+                -(ea.coarse_sch ∘ abs)
+                || H.witness ec && (ecs ec).coarse_sch && (ecs ec).fine_sch in mc,
       { admit },
       apply leads_to.trans _ P₀ P₁ },
     have Hsch' := leads_to.gen_disj' Hsch,
@@ -69,8 +72,15 @@ begin
       simp },
     simp [H₀] at Hsch',
     simp [p_or_over_p_exists_left _ _ H.witness_fis],
-    apply Hsch', },
+    apply often_imp_often.basis,
+    revert Hsch',
+    apply leads_to.strengthen_rhs,
+    apply p_exists_entails_p_exists,
+    intros e,
+    apply p_or_entails_p_or_right,
+    apply p_and_elim_left },
   { apply H.stable },
+  { admit }
 end
 
 parameters (ma : program α) (mc : program α')
@@ -80,7 +90,7 @@ structure refined : Type :=
   (ref : option mc.lbl → option ma.lbl → Prop)
   (evt_sim : ∀ ec, ⟦ mc.step_of ec ⟧
                ⟹ ∃∃ ea : { ea // ref ec ea }, ⟦ ma.step_of ea.val on abs ⟧)
-  (events : ∀ ae, evt_ref { ec // ref ec ae } mc (ma.event ae) (λ ec, mc.event ec.val) )
+  (events : ∀ ae, evt_ref_wk { ec // ref ec ae } mc (ma.event ae) (λ ec, mc.event ec.val) )
 
 parameters {ma mc}
 
@@ -102,14 +112,14 @@ end defs
 section soundness
 
 parameters {α α' β : Type}
-parameters abs : α' → α
-parameter (ma : program α)
-parameter (mc : program α')
+parameters {abs : α' → α}
+parameter {ma : program α}
+parameter {mc : program α'}
 
 open temporal
 
 parameter R : refined abs ma mc
-parameter τ : stream α'
+parameter {τ : stream α'}
 parameter M₁ : system_sem.ex mc τ
 
 section schedules
@@ -140,10 +150,26 @@ begin
   { apply abs_fine },
 end
 
-lemma conc_coarse : ∃ e', (<>[](• W e' && • CC e'.val) ) τ :=
+include R
+
+lemma evt_ref_wk.delay_sem
+: []<>(∃∃ ce, •W ce && •CC ce.val) $ τ :=
 begin
-  have H : ((∃∃ e', <>[](• W abs ma mc R e e' && • CC mc e'.val))
-                   || []<>((-•AC abs ma e) || ∃∃ e' : imp_lbl abs ma mc R e, ⟦ mc.step_of e'.val ⟧)) τ,
+  have Hdelay := (R.events e).delay,
+  have H := system_sem.often_imp_often_sem' _ M₁ Hdelay
+                (abs_coarse_and_fine M₁ e abs_coarse abs_fine),
+  clear Hdelay,
+  rw [init_p_or,inf_often_p_or,← p_not_p_imp,not_henceforth,not_eventually] at H,
+  rw [not_init,p_not_p_not_iff_self] at H,
+  have Hc := stable_entails_stable (λ _, and.left) τ abs_coarse,
+  apply H Hc,
+end
+-- lemma conc_coarse : ∃ e', (<>[](• W e' && • CC e'.val) ) τ :=
+
+lemma conc_event : ∃ e' : imp_lbl, (<>[]• CC e'.val && []<>•CF e'.val ) τ :=
+begin
+  have H : ((∃∃ e', <>[](• W R e e' && • CC e'.val))
+                   || []<>((-•AC  e) || ∃∃ e' : imp_lbl R e, ⟦ mc.step_of e'.val ⟧)) τ,
   { rw exists_action,
     apply p_or_p_imp_p_or_right _ (unless_sem_exists' M₁.safety (R.events e).stable _),
     { apply inf_often_entails_inf_often,
@@ -157,38 +183,40 @@ begin
       cases H with H₀ H₁,
       unfold program.step_of,
       rw H₁, apply H₀, },
-    have H' := leads_to.gen_disj' (R.events e).delay,
-    apply inf_often_of_leads_to (system_sem.leads_to_sem H' _ M₁),
-    simp,
-    have H' := ew_eq_true (R.events e).witness_fis,
-    rw [← p_and_over_p_exists_right],
-    simp [H'],
-    apply abs_coarse_and_fine abs ma mc _ M₁ _ abs_coarse abs_fine, },
-  simp at H,
+    have H' := (R.events e).delay,
+    have H'' := system_sem.often_imp_often_sem' _ M₁ H' , clear H',
+    rw [init_p_or, inf_often_p_or,shunting,init_exists] at H'',
+    apply evt_ref_wk.delay_sem R M₁ e abs_coarse abs_fine },
   cases H with H H,
-  { apply H },
+  { apply exists_imp_exists _ H,
+    intros ce Hcc,
+    simp, split,
+    { revert Hcc,
+      apply stable_entails_stable,
+      apply p_and_elim_right },
+    have Hc := stable_and_of_stable_of_stable Hcc abs_coarse,
+    have Ha := coincidence Hc abs_fine,
+    apply system_sem.often_imp_often_sem' _ M₁ ((R.events e).resched ce),
+    revert Ha,
+    apply inf_often_entails_inf_often,
+    intro, simp [init_p_and,W,CC,AC,AF,W,program.coarse_sch_of],
+    generalize ((•(program.event ma e).coarse_sch ∘ abs) i)  X₀,
+    generalize ((•(program.event ma e).fine_sch ∘ abs) i)    X₁,
+    generalize ((•(program.event mc (ce.val)).coarse_sch) i) X₂,
+    generalize ((•(R.events e).witness ce) i) X₃,
+    intros, begin [smt] by_cases X₀ end, },
   { exfalso,
     revert abs_coarse,
     change ¬ _,
     rw [p_not_eq_not,not_eventually,not_henceforth,p_not_p_and,p_not_p_not_iff_self],
-    apply inf_often_entails_inf_often _ _ H,
+    revert H,
+    apply inf_often_entails_inf_often,
     apply p_or_p_imp_p_or_right',
     rw p_exists_entails_eq_p_forall_entails,
     intros ec,
     apply (R.events e).sim _ , },
 end
 
-lemma conc_fine : ∀ e',
-         (<>[]•W e') τ →
-         ([]<>•CF e'.val) τ :=
-begin
-  intros e' H,
-  have H' := system_sem.leads_to_sem ((R.events e).resched e') _ M₁,
-  apply inf_often_of_leads_to H',
-  rw p_and_comm,
-  apply coincidence H,
-  apply abs_coarse_and_fine _ _ _ _ M₁ _ abs_coarse abs_fine,
-end
 
 end schedules
 
@@ -207,18 +235,14 @@ begin
     apply M₁.safety },
   { intros e COARSE₀ FINE₀,
     apply assume_neg _, intro ACT,
-    have COARSE₁ :  (<>[](•AC abs ma e && -⟦program.step_of ma e on abs⟧)) τ,
-    { rw [p_not_eq_not,not_henceforth,not_eventually] at ACT,
+    have COARSE₁ :  (<>[](•AC e && -⟦program.step_of ma e on abs⟧)) τ,
+    { rw [← inf_often_trace_action_trading] at ACT,
+      rw [← stable_trace_init_trading] at COARSE₀,
+      rw [p_not_eq_not,not_henceforth,not_eventually] at ACT,
       apply stable_and_of_stable_of_stable COARSE₀ ACT },
     clear COARSE₀ ACT,
-    cases conc_coarse abs ma mc R τ M₁ _ COARSE₁ FINE₀ with e' C_COARSE',
-    have C_COARSE : (<>[]•CC mc e'.val) τ,
-    { apply stable_entails_stable _ _ C_COARSE',
-      intro, apply and.right },
-    have WIT : (<>[]•W abs ma mc R e e') τ,
-    { apply stable_entails_stable _ _ C_COARSE',
-      intro, apply and.left },
-    have C_FINE := conc_fine abs ma mc R τ M₁ e COARSE₁ FINE₀ e' WIT,
+    cases conc_event R M₁ _ COARSE₁ FINE₀ with e' C_EVT,
+    cases C_EVT with C_COARSE C_FINE,
     rw [← inf_often_trace_trading,← action_trading],
     apply inf_often_entails_inf_often _ _ (M₁.liveness _ C_COARSE C_FINE),
     have H := (R.events e).sim e',
